theories/Syntax/BasicAst.v
@@ -5,31 +5,38 @@ Inductive sort : Set :=
 
 Definition sort_of_product (s s' : sort) := set.
 
+From Stdlib Require Logic.StrictProp.
+From LogRel Require Import Utils.
+
+
 Definition ell_list := list (prod nat bool).
 
-Fixpoint lt_ell n (ℓ : ell_list) : Prop :=
-  match ℓ with
-  | nil => True
-  | cons (n', b') ℓ => n < n' /\ (lt_ell n ℓ) 
-  end.
-
-Fixpoint ell_wf (ℓ : ell_list) : Prop :=
-  match ℓ with
-  | nil => True
-  | cons (n, b) ℓ => (lt_ell n ℓ) /\ ell_wf ℓ
-  end.
-
-Inductive SFalse : SProp := .
-Inductive STrue : SProp := SI.
+Notation SFalse := Logic.StrictProp.sEmpty.
+Notation STrue := Logic.StrictProp.sUnit.
 #[projections(primitive)]Record SAnd (A B : SProp) : SProp := Sconj { Spr1 : A;  Spr2 : B }.
 Arguments Spr1 {A B}.
 Arguments Spr2 {A B}.
 
 
+Fixpoint lt_ell n (ℓ : ell_list) : SProp :=
+  match ℓ with
+  | nil => STrue
+  | cons (pair n' b') ℓ => SAnd (Logic.StrictProp.Squash (n < n')) (lt_ell n ℓ) 
+  end.
+
+Fixpoint ell_wf (ℓ : ell_list) : SProp :=
+  match ℓ with
+  | nil => STrue
+  | cons (pair n b) ℓ => SAnd (lt_ell n ℓ) (ell_wf ℓ)
+  end.
+
+
 Definition Sis_true (b : bool) : SProp := if b then STrue else SFalse.
-From Stdlib Require Import Logic.StrictProp.
+
 
 #[projections(primitive)]Record ell : Set := {
    ℓ_list :> ell_list;
-   ℓ_wf : Squash (ell_wf ℓ_list);
+   ℓ_wf : ell_wf ℓ_list;
    }.
+
+Arguments eq_refl {_ _}, [_] _.
